lean/Hourglass.lean
@@ -3,4 +3,5 @@ import Hourglass.FunsExternal
 import Hourglass.Laws
 import Hourglass.Merge
 import Hourglass.World
+import Hourglass.Apply
 import Hourglass.Trust
